\documentclass[fleqn]{article}
\oddsidemargin 0.0in
\textwidth 6.0in
\thispagestyle{empty}
\usepackage{import}
\usepackage{amsmath}
\usepackage{graphicx}
\usepackage{flexisym}
\usepackage{amssymb}
\usepackage{bigints} 
\usepackage[english]{babel}
\usepackage[utf8x]{inputenc}
\usepackage{float}
\usepackage[colorinlistoftodos]{todonotes}

\definecolor{hwColor}{HTML}{042c4d}
\setlength\parindent{24pt}

\begin{document}

  \begin{titlepage}

    \newcommand{\HRule}{\rule{\linewidth}{0.5mm}}

    \center


    \textsc{\LARGE Arizona State University}\\[1.5cm]

    \textsc{\LARGE Advanced Calculus I }\\[1.5cm]


    \begin{figure}
      \includegraphics[width=\linewidth]{asu.png}
    \end{figure}


    \HRule \\[0.4cm]
    { \huge \bfseries Homework Four }\\[0.4cm] 
    \HRule \\[1.5cm]

    \textbf{Behnam Amiri}

    \bigbreak

    \textbf{Prof: Sergei Suslov}

    \bigbreak


    \textbf{{\large \today}\\[2cm]}

    \vfill

  \end{titlepage}

  \textbf{4.1 THE DERIVATIVE OF A FUNCTION }
  \begin{enumerate}
    \item (2) Prove that the definition of the derivative and the alternate definition of the derivative are
    equivalent.

      \textcolor{hwColor}{
        \hspace{15pt} Let's start off by remembering what the definition of the derivative and the alternate definition are.
        \\
        \\
        \textbf{The definition of the derivative:}
        \\
        The function $f$ is said to be differentiable at $x_0$ iff $\dfrac{f(x)-f(x_0)}{x-x_0}$ has a limit at $x_0$
        and we write $$f^'(x_0)=\lim\limits_{x \to x_0} \dfrac{f(x)-f(x_0)}{x-x_0}$$
        \\
        \textbf{The alternate definition of the derivative:}
        \\
        The function $f$ is said to be differentiable at $x_0$ iff $\dfrac{f(x_0+t)-f(x_0)}{t}$ has a limit at 
        zero. If this limit exists, it is called the derivative of $f$ at $x_0$.
        \\
        \\
        Even though the two definitions seem different but if we look carefully they are the same indeed.
        \\
        \\
        \emph{\textbf{Proof:}}
        \\
        \\
        Suppose $x=x_0+t$ then we can have the following:
        \\
        \\
        $
          \lim\limits_{t \to 0} \dfrac{f(x_0+t)-f(x_0)}{t}
          \\
          \\
          =\lim\limits_{x-x_0 \to 0} \dfrac{f(x)-f(x_0)}{x-x_0}
          \\
          \\
          =\lim\limits_{x \to x_0} \dfrac{f(x)-f(x_0)}{x-x_0}
          \\
          \\
          \\
          \therefore ~~~~ \lim\limits_{t \to 0} \dfrac{f(x_0+t)-f(x_0)}{t}=\lim\limits_{x \to x_0} \dfrac{f(x)-f(x_0)}{x-x_0} ~~~~~~~~~ \blacksquare
          \\
        $
      }

    \item (3) Use the definition to find the derivative of $f(x)=\sqrt{x}$, for $x > 0$. Is $f$ differentiable at zero? Explain.

      \textcolor{hwColor}{
        \\
        The definiton is defined as $f^'(x_0)=\lim\limits_{x \to x_0} \dfrac{f(x)-f(x_0)}{x-x_0}$ we have:
        \\
        \\
        $
          f^'(x_0)=\lim\limits_{x \to 0} \dfrac{f(x)-f(0)}{x-0}
          \\
          \\
          =\lim\limits_{x \to x_0} \dfrac{\sqrt{x}-\sqrt{0}}{x-0}
          \\
          \\
          =\lim\limits_{x \to x_0} \dfrac{\sqrt{x}}{x}
          \\
          \\
        $
        With the help of L’H\^{o}pital’s Rule we have:
        \\
        \\
        $
          =\lim\limits_{x \to x_0} \dfrac{\dfrac{1}{2\sqrt{x}}}{1}
          \\
          \\
          =\dfrac{1}{2\sqrt{x_0}}
          \\
          \\
          \\
          \therefore ~~~~ f^'(0)=+\infty ~~~~ \checkmark 
        $
        \\
        \\
        It is not differentiable, because the derivative of $f$ at zero tends to $+\infty$ as it was shown. 
        By using the alternate definition of the derivative we have:
        \\
        \\
        $
          f^'(x_0)=\lim\limits_{t \to 0} \dfrac{f(x_0+t)-f(x_0)}{t}
          \\
          \\
          =\lim\limits_{t \to 0} \dfrac{\sqrt{x_0+t}-\sqrt{x_0}}{t}
          \\
          \\
          =\lim\limits_{t \to 0} \dfrac{\sqrt{x_0+t}-\sqrt{x_0}}{t} \times \dfrac{\sqrt{x_0+t}+\sqrt{x_0}}{\sqrt{x_0+t}+\sqrt{x_0}}
          \\
          \\
          =\lim\limits_{t \to 0} \dfrac{x_0+t-x_0}{t \left(\sqrt{x_0+t}+\sqrt{x_0}\right)}
          \\
          \\
          =\lim\limits_{t \to 0} \dfrac{t}{t\left(\sqrt{x_0+t}+\sqrt{x_0}\right)}
          \\
          \\
          =\lim\limits_{t \to 0} \dfrac{1}{\sqrt{x_0+t}+\sqrt{x_0}}
          \\
          \\
          =\dfrac{1}{2\sqrt{x_0}}
          \\
          \\
          \\
          \therefore ~~~~ f^'(0)=+\infty ~~~~ \checkmark 
        $
        \\
        \\
        As we expected we got the same result which is function $f$ is not differentiable at zero. $~~~~ \checkmark$
        \\
      }

    \item (4) Use the definition to find the derivative of $g(x)=x^2$.

      \textcolor{hwColor}{
        We know the definition is $g^'(x_0)=\lim\limits_{t \to 0} \dfrac{f(x_0+t)-f(x_0)}{t}$ and $g(x)=x^2$ so
        we have the following:
        \\
        \\
        $
          g^'(x_0)=\lim\limits_{t \to 0} \dfrac{f(x_0+t)-f(x_0)}{t}
          \\
          \\
          =\lim\limits_{t \to 0} \dfrac{\left(x_0+t\right)^2-x_0^2}{t}
          \\
          \\
          =\lim\limits_{t \to 0} \dfrac{x_0^2+2x_0t+t^2-x_0^2}{t}
          \\
          \\
          =\lim\limits_{t \to 0} \dfrac{t \left(2x_0+t\right)}{t}
          \\
          \\
          =\lim\limits_{t \to 0} 2x_0+t
          \\
          \\
          \\
          \therefore ~~~~ g^'(x_0)=2x_0 ~~~~ \checkmark
        $
      }

    \item (6) Suppose $f: (a, b) \longrightarrow R$ is differentiable at $x \in (a, b)$. Prove that 
    $$
      \lim\limits_{h \to 0} \dfrac{f(x+h)-f(x-h)}{2h}
    $$
    exists and equals $f^'(x)$. Give an example of a function where this limit exists, but the
    function is not differentiable.

      \textcolor{hwColor}{
        According to the textbook, a function $f$ is said to be differentiable at $x_0$ or has
        a derivative at $x_0$ iff $\lim\limits_{t \to 0} \dfrac{f(x_0+t)-f(x_0)}{t}$ exists at $x_0$.
        \\
        \\
        So let's start with the given statement to see where it can take us.
        \\
        \\
        $
          \lim\limits_{h \to 0} \dfrac{f(x+h)-f(x-h)}{2h}
          \\
          \\
          =\lim\limits_{h \to 0} \dfrac{f(x+h)-f(x-h)+f(x)-f(x)}{2h}
          \\
          \\
          =\lim\limits_{h \to 0} \left[\dfrac{f(x+h)-f(x)}{2h}+\dfrac{-f(x-h)+f(x)}{2h}\right]
          \\
          \\
          =\lim\limits_{h \to 0} \left[\dfrac{f(x+h)-f(x)}{2h}+\dfrac{f(x-h)-f(x)}{-2h}\right]
          \\
          \\
          =\dfrac{1}{2} \left[\lim\limits_{h \to 0}\dfrac{f(x+h)-f(x)}{h}+\lim\limits_{h \to 0}\dfrac{f(x-h)-f(x)}{-h}\right]
          \\
          \\
          =\dfrac{1}{2} \left[f^'(x)+f^'(x)\right]
          \\
          \\
          \\
          \therefore ~~~~ \lim\limits_{h \to 0} \dfrac{f(x+h)-f(x-h)}{2h} \Longleftrightarrow f^'(x) ~~~~ \checkmark
        $
        \\
        \\
        \\
        An example of a function that is continuous but non differentiable at zero is $f(x)=|x|$.
        \\
        \\
        $
          \lim\limits_{h \to 0} \dfrac{f(0+h)-f(0-h)}{2h}
          \\
          \\
          =\lim\limits_{h \to 0} \dfrac{|0+h|-|0-h|}{2h}
          \\
          \\
          \\
          \therefore ~~~~ \lim\limits_{h \to 0} \dfrac{f(0+h)-f(0-h)}{2h}=0
        $
        \\
        \\
        Based off of the result, the limit of $f$ at $x=0$ is zero. (its limit exists) but $f$ is not differentiable at zero.
        \\
        \\
        \includegraphics[height=5cm, width=9cm]{absoluteValueFunction.JPG}
      }


  \end{enumerate}

  \rule{15cm}{1pt}

  \textbf{4.2  THE ALGEBRA OF DERIVATIVES}
  \begin{enumerate}
    \item (11) Prove $f: (0, 1) \longrightarrow R$ defined by $f(x)=\sqrt{2x^2-3x+6}$ is differentiable on $(0, 1)$ and 
    compute the derivative.

      \textcolor{hwColor}{
        On page $119$ of the textbook, we learned that \emph{If $f$ is differentiable at $x_0$ and $g$ is differentiable at $f(x_0)$, then $gof$ is differentiable at $x_0$}.
        (Chain rule)
        $$
          \left(gof\right)^'(x_0)=g^'\left(f(x_0)\right) f^'(x_0)
        $$
        Let's assume $g(x)=2x^2-3x+6$ and $w(x)=\sqrt{x}$. We know that both $g(x)$ and $w(x)$ are differentiable, so does 
        their composition $\left(gow\right)$ therefore:
        \\
        \\
        $
          f^'(x)=\dfrac{d}{dx}(gow)
          \\
          \\
          =\dfrac{d}{dx} g\left(w(x)\right)
          \\
          \\
          =\dfrac{d}{dx} \left(2x^2-3x+6\right) \times \dfrac{d}{dx} \left(\sqrt{2x^2-3x+6}\right)
          \\
          \\
          =\left(4x-3\right) \times \dfrac{1}{2\sqrt{2x^2-3x+6}}
          \\
          \\
          \\
          \therefore ~~~~ f^'(x)=\dfrac{4x-3}{2\sqrt{2x^2-3x+6}} ~~~~ \checkmark
        $
      }

    \item (14) Suppose $f: R \longrightarrow R$ is differentiable and define $g(x)=x^2 f(x^3)$. Show that $g$ is
    differentiable and compute $g^'$.

      \textcolor{hwColor}{
        On page $119$ of the textbook, we learned that \emph{If $f$ is differentiable at $x_0$ and $g$ is differentiable at $f(x_0)$, then $gof$ is differentiable at $x_0$}.
        (Chain rule)
        $$
          \left(gof\right)^'(x_0)=g^'\left(f(x_0)\right) f^'(x_0)
        $$
        The composition of two differentiable functions is also differentiable. We know $x^3$ is differentiable and by the chain rule $f(x^3)$ is differentiable too.
        \\
        \\
        $
          \left(f(x^3)\right)^'
          =\dfrac{d}{dx}x^3 \times f^'(x^3)
          =3x^2 f^'(x^3)
        $
        \\
        \\
        Now we are ready to find $g^'(x)$.
        \\
        \\
        $
          g^'(x)=\dfrac{d}{dx}(x^2) f(x^3)+x^2\dfrac{d}{dx} \left(f(x^3)\right)^
          =2x f(x^3)+x^2 \left[3x^2 f^'(x^3)\right]
          \\
          \\
          \\
          \therefore ~~~~ g^'(x)=2x f(x^3)+3x^4 f^'(x^3) ~~~~ \checkmark
          \\
        $
      }
    
    \item (15) Define $f(x)=\sqrt{x+\sqrt{x+\sqrt{x}}}$ for $x \geq 0$. Determine where $f$ is differentiable and compute
    the derivative. 

      \textcolor{hwColor}{
        \emph{We know that $\sqrt{x}$ is differentiable.}
        \\
        \\
        We can find the derivative of the given function by the chain and addition rules.
        \\
        \\
        $
          \dfrac{df}{dx}=\dfrac{d}{dx} \left[\sqrt{x+\sqrt{x+\sqrt{x}}}\right]
          \\
          \\
          =\dfrac{d}{dx} \left[\left(x+\sqrt{x+\sqrt{x}}\right)^{\dfrac{1}{2}}\right]
          \\
          \\
          =\dfrac{1}{2} \times \dfrac{d}{dx} \left(x+\sqrt{x+\sqrt{x}}\right) \times \left(x+\sqrt{x+\sqrt{x}}\right)^{-\dfrac{1}{2}} ~~~~~ (A)
          \\
          \\
        $
        Now let's find the derivative of $\dfrac{d}{dx} \left(x+\sqrt{x+\sqrt{x}}\right)$ then we can plug it into equation $(A)$.
        \\
        \\
        $
          \dfrac{d}{dx} \left(x+\sqrt{x+\sqrt{x}}\right)
          \\
          \\
          =\dfrac{d}{dx} \left[x+\left(x+\sqrt{x}\right)^{\dfrac{1}{2}}\right]
          \\
          \\
          =1+\dfrac{1}{2} \dfrac{d}{dx} \left[x+\sqrt{x}\right] \left(x+\sqrt{x}\right)^{-\dfrac{1}{2}}
          \\
          \\
          =1+\dfrac{1}{2} \left(1+\dfrac{1}{2\sqrt{x}}\right) \left(x+\sqrt{x}\right)^{-\dfrac{1}{2}}
          \\
          \\
          \\
          \\
          \therefore ~~~~ (A) ~~~~  \dfrac{1}{2} \times \left[1+\dfrac{1}{2} \left(1+\dfrac{1}{2\sqrt{x}}\right) \left(x+\sqrt{x}\right)^{-\dfrac{1}{2}}\right] \times \left(x+\sqrt{x+\sqrt{x}}\right)^{-\dfrac{1}{2}}
          \\
          \\
          \\
          =\dfrac{1}{2 \sqrt{x+\sqrt{x+\sqrt{x}}}}+\dfrac{\left(1+\dfrac{1}{2\sqrt{x}}\right)}{4 \left(x+\sqrt{x+\sqrt{x}}\right)^{\dfrac{1}{2}} \left(x+\sqrt{x}\right)^{\dfrac{1}{2}}}
          \\
          \\
          \\
          \therefore ~~~~ \dfrac{df}{dx}=\dfrac{1}{2 \sqrt{x+\sqrt{x+\sqrt{x}}}}+\dfrac{1+\dfrac{1}{2\sqrt{x}}}{4 \sqrt{x+\sqrt{x+\sqrt{x}}} \sqrt{x+\sqrt{x}}} ~~~~ \checkmark
          \\
        $
      }

  \end{enumerate}

  \rule{15cm}{1pt}

  \textbf{4.3 ROLLE'S THEOREM AND THE MEAN-VALUE THEOREM}
  \begin{enumerate}
    \item (16) Define $f: [0, 2] \longrightarrow R$ by $f(x)=\sqrt{2x-x^2}$. Show that $f$ satisfies the conditions of Rolle's
    theorem and find $c$ such that $f^'(c)=0$.

      % \textcolor{hwColor}{

      % }

    \item (17) Define $f: R \longrightarrow R$ by $f(x)=\dfrac{1}{1+x^2}$. Prove that $f$ has a maximum value and find the
    point at which that maximum occurs.

      % \textcolor{hwColor}{

      % }

    \item (28) Prove that the function $f(x)=2x^3+3x^2-36x+5$ is $1-1$ on the interval $[-1,1]$. Is $f$ increasing or decreasing?

      % \textcolor{hwColor}{

      % }

  \end{enumerate}

  \rule{15cm}{1pt}

  \textbf{4.4 L'HOSPITAL'S RLILE AND THE INVERSE-FUNCTION THEOREM}
  \begin{enumerate}
    \item Assume the rules for differentiating the elementary functions, and use L'Hospital's Rule
    and find the following limits: 
    \begin{enumerate}
      \item $\lim\limits_{x \to 1} \dfrac{ln(x)}{x-1}$

        % \textcolor{hwColor}{

        % }

      \item $\lim\limits_{x \to 0} \dfrac{x}{e^x-1}$

        % \textcolor{hwColor}{

        % }

      \item $\lim\limits_{x \to 0} \dfrac{sin(x)}{x}$

        % \textcolor{hwColor}{

        % }

    \end{enumerate}

    \item (33) Use L'Hospitd's Rule to find the limit:
    $$
      \lim\limits_{x \to 0} \dfrac{x^2 sin(x)}{sin(x)-x cos(x)}
    $$

      % \textcolor{hwColor}{

      % }

    \item (39) Suppose $f: R \longrightarrow R$ is such that $f(x+y)=f(x)f(y), f$ is differentiable at zero, and $f$ is
    not identically zero. Prove that $f$ is differentiable everywhere and that $f^'(x)=f(x)f^'(0)$.
    Assuming the properties of the exponential function, prove that $f(x)=e^{cx}$ where $c=f^'(0)$.

      % \textcolor{hwColor}{

      % }

  \end{enumerate}
\end{document}
